initialize_normal

src/locations.v
@@ -16,15 +16,18 @@ Context `{Countable RefinementIndex}.
 Context `{EqDecision RefinementIndex}.
 Context (ref_map : RefinementIndex -> Refinement M M).*)
 
-Class RefinementIndex (M: Type) `{!EqDecision M} `{!TPCM M} (RI: Type) :=
-    refinement_of : RI -> Refinement M M .
+Class RefinementIndex (M: Type) `{!EqDecision M} `{!TPCM M} (RI: Type) := {
+    refinement_of : RI -> Refinement M M;
+    triv_ri : RI;
+}.
+Global Arguments triv_ri {M}%type_scope {EqDecision0 TPCM0} _ {RefinementIndex}.
 
 Inductive Loc (RI: Type) `{!EqDecision RI, !Countable RI} :=
   | BaseLoc : nat -> Loc RI
   | ExtLoc : nat -> RI -> Loc RI -> Loc RI
   | CrossLoc : Loc RI -> Loc RI -> Loc RI
 .
-Arguments BaseLoc {RI}%type_scope {EqDecision0 Countable0} _%nat_scope.
+Arguments BaseLoc _%type_scope {EqDecision0 Countable0} _%nat_scope.
 Arguments ExtLoc {RI}%type_scope {EqDecision0 Countable0} _%nat_scope _ _.
 Arguments CrossLoc {RI}%type_scope {EqDecision0 Countable0} _ _.
 
@@ -34,6 +37,9 @@ Proof. solve_decision. Defined.
 Global Instance loc_countable RI `{!EqDecision RI} `{!Countable RI} : Countable (Loc RI). Admitted.
 
 Definition nat_of_extstep {RI} `{!EqDecision RI, !Countable RI} (alpha:nat) (ri: RI) : nat.
+Admitted.
+
+Definition nat_of_basestep RI `{!EqDecision RI, !Countable RI} (alpha:nat) : nat.
 Admitted.
 
 Definition pls_of_loc {RI} `{!EqDecision RI} `{!Countable RI} (loc: Loc RI) : (listset PathLoc). Admitted.
